\begin{figure}
  \begin{center}
    \[
      \begin{array}{l}
        \mfun{types}(Σ) = \{ T \bnfalt C : τ_1 * … * τ_m → T ∈ Σ \} \\
        \mrmatch^s(Σ; Γ; τ; Χ; 0) = \{ \} \\
        \mrmatch^s(Σ; Γ; τ; Χ; k) = \displaystyle{\bigcup_{\scriptstyle T ∈ \mfun{types}(Σ)}}
        \⇥{1} \{ \underline{\mmatch\;E\;\mwith\;\many{p_i → ◼_i}{i < m}} \bnfalt \\
        \⇥{2}   E ∈ \mgen_E(Σ; Γ; T; s), \\
        \⇥{2}   \many{(p_i, Χ_i)}{i < m} = \mfun{distribute}(Σ, T, Χ, E), \\
        \⇥{2}   \many{Γ_i}{i < m} = \mfun{binders}(Γ, E, p_i), \\
        \⇥{2}   \many{◼_i = \mrtree^s(Σ; Γ_i, Γ; τ; Χ_i; k-1)}{i < m} \} \\
        \\
        \mrtree^s(Σ; Γ; τ_1 → τ_2; Χ; k) = \{ \underline{\mfix\;f\;(x{:}τ_1) : τ_2 = ◼} \bnfalt \\
        \⇥{1} Χ' = \mfun{apply}(f, x, σ_1 ↦ \mpf_1) \concat … \concat \mfun{apply}(f, x, σ_n ↦ \mpf_n), \\
        \⇥{1} ◼ = \mrtree^s(Σ; f{:}τ_1 → τ_2 \{\mrec\}, x{:}τ_1 \{\marg{f}\}; Γ; Χ'; k) \\
        \} \\
        \⇥{1} \text{where} \\
        \⇥{2}   Χ = σ_1 ↦ \mpf_1, …, σ_n ↦ \mpf_n \\
        \\
        \mrtree^s(Σ; Γ; T; Χ; k) = \{ \underline{C(◼_1, …, ◼_m)} \bnfalt \\
        \⇥{1}   Χ_1, …, Χ_m = \mfun{proj}(X), \\
        \⇥{1}   \many{◼_i ∈ \mrtree^s(Σ; Γ; τ_i; Χ_i; k)}{i < m} \\
        \} ∪ \mrmatch^s(Σ; Γ; τ; Χ; k) \\
        \text{where} \\
        \⇥{1}   Χ = \many{σ_i ↦ C(I_{i1}, …, C_{im})}{i < n} \\
        \⇥{1}   C : τ_1 * … * τ_m ∈ Σ \\
        \\
        \mguess(Σ; Γ; τ; Χ; 0) = \{ \} \\
        \mguess(Σ; Γ; τ; Χ; k) = \{ E \bnfalt E ∈ \mgen_E(Σ; Γ; τ; k), E ⊨ Χ \} \\
      \end{array}
    \]
  \end{center}
  \hrule
  \caption{Refinement tree creation and $E$-guessing}
  \label{fig:app-implementation-refinement-tree}
\end{figure}

\begin{figure}[!t]
  \centering \fbox{$\mgen_E(Σ; Γ; τ; n)$}
  \begin{align*}
    \mgen_E(Σ; ·; τ; n)  &= \{ \} \\
    \mgen_E(Σ; ·; τ; 0)  &= \{ \} \\
    \mgen_E(Σ; x{:}τ_1,Γ; τ; n) &= \mgen_E^{x{:}τ_1}(Σ; Γ; τ; n) ∪ \mgen_E(Σ; Γ; τ; n)
  \end{align*}

  \centering \fbox{$\mgen_E^{x{:}τ_1}(Σ; Γ; τ; n)$}
  \begin{align*}
    \mgen_E^{x{:}τ_1}(Σ; Γ; τ; 0) & = \{ \} & & \\
    \mgen_E^{x{:}τ}(Σ; Γ; τ; 1)   & =  \{ x \} & & \\
    \mgen_E^{x{:}τ_1}(Σ; Γ; τ; 1) & =  \{ \} \qquad (τ ≠ τ_1) & & \\
    \mgen_E^{x{:}τ_1}(Σ; Γ; τ; n) & =  \bigcup_{τ_2 → τ ∈ Γ} \bigcup_{k = 1}^{n - 1} & &
  \end{align*}
  \[
  \begin{array}{llcl}
         & (\mgen_E^{x{:}τ_1}(Σ; Γ; τ_2 → τ; k) & \appprod & \mgen_I(Σ; Γ; τ_2; n-k)) \\
    \cup & (\mgen_E(Σ; Γ; τ_2 → τ; k)           & \appprod & \mgen_I^{x:τ_1}(Σ; Γ; τ_2; n-k)) \\
    \cup & (\mgen_E^{x{:}τ_1}(Σ; Γ; τ_2 → τ; k) & \appprod & \mgen_I^{x:τ_1}(Σ; Γ; τ_2; n-k)) \\
  \end{array}
  \]
  \hrule
  \caption{Relevant $E$-term generation}
  \label{fig:app-implementation-genE}
\end{figure}

\begin{figure}[!t]
  \centering \fbox{$\mgen_I(Σ, Γ, τ, n)$}
  \begin{gather*}
    \begin{split}
      \mgen_I(Σ; ·; τ; n)       &= \{ \} \\
      \mgen_I(Σ; Γ; τ; 0)       &= \{ \} \\
      \mgen_I(Σ; x:τ_1,Γ; τ; n) &= \mgen_I^{x:τ_1}(Σ; Γ; τ; n) ∪ \mgen_I(Σ; Γ; τ; n) \\
    \end{split} \\
    \begin{array}{l}
      \mgen_I(Σ; ·; τ_1 → τ_2; n) = \\
        \⇥{1}\{ \mfix\;f\;(x{:}τ_1) : τ_2 = I \bnfalt I ∈ \mgen_I(Σ; f:τ_1 → τ_2, x:τ_1; τ_2; n-1) \} \\
    \end{array} \\
    \begin{split}
      \mgen_I^{x:τ}(Σ; Γ; T; n) &= \mgen_E^{x:τ}(Σ; Γ; T; n) \\
        & \bigcup_{\scriptstyle C:τ_1 * … * τ_k → T ∈ Σ}
          \bigcup_{\begin{array}{c}\scriptstyle n_1, …, n_k\;\text{for} \\ \scriptstyle n_1 + … + n_k = n\end{array}} \\
        & \{ C(I_1, …, I_k) \bnfalt I_j ∈ \mgen_I(Σ; Γ; τ_j; n_j) \}
    \end{split}
  \end{gather*}

  \centering \framebox{\mbox{$\mgen_I^{x:τ_1}(Σ; Γ; τ; n)$}}
  \begin{multline*}
    \mgen_I^{x:τ}(Σ; Γ; τ_1 → τ_2; n) = \mgen_E^{x:τ}(Σ; Γ; τ_1 → τ_2; n)\;∪ \\
    \{ \mfix\;f\;(y{:}τ_1) : τ_2 = I \bnfalt I ∈ \mgen_I^{x:τ}(Σ; f:τ_1 → τ_2, y:τ_1, Γ; τ_2; n-1) \}
  \end{multline*}
  \begin{gather*}
    \begin{split}
      \mgen_I^{x:τ}(Σ; Γ; T; n) &= \mgen_E^{x:τ}(Σ; Γ; T; n) \\
        & \bigcup_{\scriptstyle C : τ_1 * … * τ_k → T ∈ Σ}
          \bigcup_{\begin{array}{c}\scriptstyle n_1, …, n_k\;\text{for} \\ \scriptstyle n_1 + … + n_k = n\end{array}}
          \bigcup_{\begin{array}{c}\scriptstyle r_1, …, r_k ∈ \\ \scriptstyle \mfun{parts}(k)\end{array}} \\
            & \{ C(I_1, …, I_k) \bnfalt I_j ∈ \mfun{genp}_I^{m_j; x:τ}(Σ; Γ; τ_j; n_j) \}
    \end{split} \\[11pt]
    \mfun{parts}(k) = \{ \underbrace{\mathsf{Not}, …, \mathsf{Not}}_{i-1},
                        \mathsf{Must},
                        \underbrace{\mathsf{May}, …, \mathsf{May}}_{k-i}
                        \bnfalt i ∈ 1, …, k \} \\
    \mfun{genp}_I^{r; x:τ_1}(Σ; Γ; τ; n) = \begin{cases}
      \mgen_I^{x:τ_1}(Σ; Γ; τ; n) & r = \mathsf{Must} \\
      \mgen_I(Σ; x:τ_1, Γ; τ; n)  & r = \mathsf{May}  \\
      \mgen_I(Σ; Γ; τ; n)         & r = \mathsf{Not}  \\
    \end{cases}
  \end{gather*}
  \hrule
  \caption{Relevant $I$-term generation}
  \label{fig:app-implementation-genI}
\end{figure}
