\begin{figure}
  \begin{center}
    \begin{tabular}{>{$}l<{$} >{$}r<{$} >{$}l<{$} l}
      τ  & \bnfdef & τ_1 → τ_2 \bnfalt T & Types\\
      e  & \bnfdef & x \bnfalt e_1\,e_2 \bnfalt λx{:}τ.\,e \bnfalt c & Terms \\
      v  & \bnfdef & λx{:}τ.\,e \bnfalt c & Values \\
      ℰ  & \bnfdef & ◻ \bnfalt ℰ\,e \bnfalt v\,ℰ & Evaluation Contexts \\
      Γ  & \bnfdef & · \bnfalt x{:}τ, Γ & Typing Contexts \\
      \\
      E  & \bnfdef & x \bnfalt E\,I & Elimination Terms \\
      I  & \bnfdef & E \bnfalt λx{:}τ.\,I \bnfalt c & Introduction Terms \\
      σ  & \bnfdef & · \bnfalt [v/x]σ & Evaluation Environments \\
      χ  & \bnfdef & c \bnfalt \mpf & Example Values \\
      \mpf & \bnfdef & \many{v_i ⇒ χ_i}{i < m} & Partial Functions \\
      Χ  & \bnfdef & · \bnfalt σ ↦ χ, Χ &  Example Worlds
    \end{tabular} \\[12pt]
    \hrule
    \begin{gather*}
      \fbox{$Γ ⊢ e : τ$}\;\fbox{$e⟶ e'$} \qquad
        \text{(Same as \stlc{})} \\
      \fbox{$Γ ⊢ E ⇒ τ$} \qquad
        \inferrule[t-Evar]
          {x:τ ∈ Γ}
          {Γ ⊢ x ⇒ τ} \qquad
        \inferrule[t-Eapp]
          {Γ ⊢ E ⇒ τ_1 → τ_2 \\ Γ ⊢ I ⇐ τ_1}
          {Γ ⊢ E\;I ⇒ τ_2} \\
      \fbox{$Γ ⊢ I ⇐ τ$} \qquad
        \inferrule[t-Ilam]
          {x{:}τ_1, Γ ⊢ I ⇐ τ_2}
          {Γ ⊢ λx{:}τ_1.\;I ⇐ τ_1 → τ_2} \qquad
        \inferrule[t-Ibase]
          { }
          {Γ ⊢ c ⇐ T} \qquad
        \inferrule[t-Ielim]
          {Γ ⊢ E ⇒ τ}
          {Γ ⊢ E ⇐ τ} \\
      \fbox{$Γ ⊢ χ : τ$} \qquad
        \inferrule[t-ex-base]
          { }
          {Γ ⊢ c : T} \qquad
        \inferrule[t-ex-pf]
          {\many{Γ ⊢ v_i : τ_1}{i < m} \\ \many{Γ ⊢ χ_i : τ_2}{i < m}}
          {Γ ⊢ \many{v_i ⇒ χ_i}{i < m} : τ_1 → τ_2} \\
      \fbox{$Γ ⊢ σ$} \qquad
        \inferrule[t-env-empty]
          { }
          {Γ ⊢ ·} \qquad
        \inferrule[t-env-cons]
          {x{:}τ ∈ Γ \\ ⊢ v : τ \\ Γ ⊢ σ}
          {Γ ⊢ [v/x]σ} \\
      \fbox{$Γ ⊢ Χ : τ$} \qquad
        \inferrule[t-exw-empty]
          { }
          {Γ ⊢ · : τ} \qquad
        \inferrule[t-exw-cons]
          {Γ ⊢ σ \\ ∀x{:}τ ∈ Γ.\,∃v.\,[x/v] ∈ σ \\\\ Γ ⊢ χ : τ \\ Γ ⊢ Χ : τ}
          {Γ ⊢ σ ↦ χ, Χ : τ}
    \end{gather*}
  \end{center}

  \hrule
  \caption{\lsyn{} syntax and typechecking}
  \label{fig:lsyn-defn}
\end{figure}
