\begin{figure}
  \begin{center}
    \begin{tabular}{>{$}l<{$} >{$}r<{$} >{$}l<{$}}
      τ  & \bnfdef & … \bnfalt τ_1 + τ_2 \\
      e  & \bnfdef & … \bnfalt \mmatch\;e\;\mwith\;\minl{x_1} → e_1 \semisep \minr{x_2} → e_2 \bnfalt \minl{e} \bnfalt \minr{e} \\
      v  & \bnfdef & … \bnfalt \minl{v} \bnfalt \minr{v} \\
      ℰ  & \bnfdef & … \bnfalt \mmatch\;ℰ\;\mwith\;\minl{x_1} → e_1 \semisep \minr{x_2} → e_2 \\
      E  & \bnfdef & … \\
      I  & \bnfdef & … \bnfalt \mmatch\;E\;\mwith\;\minl{x_1} → I_1 \semisep \minr{x_2} → I_2 \bnfalt \minl{I} \bnfalt \minr{I} \\
      χ  & \bnfdef & … \bnfalt \minl{χ} \bnfalt \minr{χ} \\
    \end{tabular} \\[12pt]
    \hrule
    \begin{gather*}
      \fbox{$Γ ⊢ e : τ$} \qquad
        \inferrule[t-inl]
          {Γ ⊢ e : τ_1}
          {Γ ⊢ \minl{e} : τ_1 + τ_2} \qquad
        \inferrule[t-inr]
          {Γ ⊢ e : τ_2}
          {Γ ⊢ \minr{e} : τ_1 + τ_2} \\
        \inferrule[t-match]
          {Γ ⊢ e : τ_1 + τ_2 \\\\
           x_1{:}τ_1, Γ ⊢ e_1 : τ \\ x_2{:}τ_2, Γ ⊢ e_2 : τ}
          {Γ ⊢ \mmatch\;e\;\mwith\;\minl{x_1} → e_1 \semisep \minr{x_2} → e_2 : τ} \\
      \fbox{$Γ ⊢ I ⇐ τ$} \qquad
        \inferrule[t-Iinl]
          {Γ ⊢ I ⇐ τ_1}
          {Γ ⊢ \minl{I} ⇐ τ_1 + τ_2} \qquad
        \inferrule[t-Iinr]
          {Γ ⊢ I ⇐ τ_2}
          {Γ ⊢ \minr{I} ⇐ τ_1 + τ_2} \\
        \inferrule[t-Imatch]
          {Γ ⊢ E ⇒ τ_1 + τ_2 \\\\
           x_1{:}τ_1, Γ ⊢ I_1 ⇐ τ \\ x_2{:}τ_2, Γ ⊢ I_2 ⇐ τ}
          {Γ ⊢ \mmatch\;E\;\mwith\;\minl{x_1} → I_1 \semisep \minr{x_2} → I_2 : τ} \\
      \fbox{$Γ ⊢ χ : τ$} \qquad
        \inferrule[t-ex-inl]
          {Γ ⊢ χ : τ_1}
          {Γ ⊢ \minl{χ} : τ_1 + τ_2} \qquad
        \inferrule[t-ex-inr]
          {Γ ⊢ χ : τ_2}
          {Γ ⊢ \minr{χ} ⇐ τ_1 + τ_2} \\
      \fbox{$e ⟶ e'$} \qquad
        \inferrule[eval-match-inl]
          {}
          {\mmatch\;\minl{v}\;\mwith\;\minl{x_1} → e_1 \semisep \minr{x_2} → e_2 ⟶ [v/x_1]e_1} \\
        \inferrule[eval-match-inr]
          {}
          {\mmatch\;\minr{v}\;\mwith\;\minl{x_1} → e_1 \semisep \minr{x_2} → e_2 ⟶ [v/x_2]e_2}
    \end{gather*}
  \end{center}
  \hrule
  \caption{\lsyn{} sums definitions}
  \label{fig:lsyn-sums-defn}
\end{figure}
