\begin{figure}
  \begin{center}
    \begin{gather*}
      \fbox{$Σ;Γ ⊢ τ ⇝ E$} \qquad
        \inferrule[eguess-var]
          {x{:}τ ∈ Γ}
          {Σ;Γ ⊢ τ ⇝ x} \qquad
        \inferrule[eguess-app]
          {Σ;Γ ⊢ τ_1 → τ_2 ⇝ E \\
           Σ;Γ ⊢ τ_1 ▷ · ⇝ I \\\\
           \mfun{struct}(Γ, E, I)}
          {Σ;Γ ⊢ τ_2 ⇝ E\;I} \\
      \fbox{$I ⊨ Χ$} \qquad
        \inferrule[satisfies]
        {∀σ ↦ χ ∈ Χ.\, σ(I) ⟶^* v ∧ v ≃ χ}
        {I ⊨ Χ} \\
      \fbox{$Σ;Γ ⊢ τ ▷ Χ ⇝ I$} \qquad
        \inferrule[irefine-guess]
          {Σ;Γ ⊢ τ ⇝ E \\ E ⊨ Χ}
          {Σ;Γ ⊢ τ ▷ Χ ⇝ E} \qquad
        \inferrule[irefine-unit]
          {Χ = \many{σ_i ↦ ()}{i < n}}
          {Σ;Γ ⊢ \munit ▷ Χ ⇝ ()} \\
        \inferrule[irefine-base]
        {C : τ_1, …, τ_k → T ∈ Σ \\ X = \many{σ_i ↦ C(I_{i1}, …, I_{ik})}{i < n} \\\\
         \mfun{proj}(X) = C_1, …, C_k \\ \many{Σ;Γ ⊢ I_i ⇐ τ_i}{i < k}}
          {Σ;Γ ⊢ T ▷ Χ ⇝ C\;(I_1, …, I_k) ⇐ T} \\
        \inferrule[irefine-arr]
          {X = σ_1 ↦ pf_1, …, σ_n ↦ pf_n \\\\
           X' = \mfun{apply}(f, x, σ_1 ↦ pf_1) \concat … \concat \mfun{apply}(f, x, σ_n ↦ pf_n) \\\\
           Σ;f{:}τ_1 → τ_2 \{\mrec\}, x{:}τ_1 \{\marg{f}\}, Γ ⊢ I ▷ X' ⇝ τ_2}
          {Σ;Γ ⊢ τ_1 → τ_2 ▷ Χ ⇝ \mfix\;f\;(x{:}τ_1) : τ_2 = I} \\
        \inferrule[t-match]
          {Σ;Γ ⊢ T ⇝ E \\ \mfun{distribute}(Σ, T, X, E) = \many{(p_i, X'_i)}{i < m} \\\\
          \many{\mfun{binders}(Γ, E, p_i) = Γ_i}{i < m} \\ \many{Σ; Γ_i, Γ ⊢ τ ▷ Χ ⇝ I_i}{i < m}}
          {Σ;Γ ⊢ τ ▷ Χ ⇝ \mmatch\;E\;\mwith\;\many{p_i → e_i}{i < m}}
    \end{gather*}
  \end{center}
  \hrule
  \caption{\mlsyn{} synthesis}
  \label{fig:mlsyn-synthesis}
\end{figure}
