\begin{figure}
  \begin{center}
    \begin{gather*}
      \fbox{$e → e'$} \qquad
        \inferrule[eval-ctx]
          {e ⟶ e'}
          {ℰ[e] ⟶ ℰ[e']} \qquad
        \inferrule[eval-nomatch]
          {}
          {ℰ[\mNoMatch] ⟶ \mNoMatch} \qquad
        \inferrule[eval-app]
          {}
          {(λx{:}τ.\,e)\;v ⟶ [v/x]e} \\
        \inferrule[eval-pf-good]
          {v ≃ v_j \\ j ∈ 1, …, m}
          {(\many{v_i ⇒ χ_i}{i < m})\;v → χ_j} \qquad
        \inferrule[eval-pf-bad]
          {∀i ∈ 1, …, m.\,v ≄ v_i}
          {(\many{v_i ⇒ χ_i}{i < m})\;v → \mNoMatch}
    \end{gather*}
    \[
      \begin{array}{l}
        \rulename{eval-match} \\
        \quad \mmatch\;C(v_1, …, v_k)\;\mwith\;p_1 → e_1 \bnfalt … \bnfalt C(x_1, …, x_k) → e \bnfalt … \bnfalt p_m → e_m \\
        \qquad ⟶ [v_1/x_1]…[v_k/x_k](e)
      \end{array}
    \]
    \begin{gather*}
      \fbox{$v ≃ v'$} \qquad
        \inferrule[eq-refl]
          {}
          {v ≃ v} \qquad
        \inferrule[eq-sym]
          {v' ≃ v}
          {v ≃ v'} \\
        \inferrule[eq-pf-pf]
          {∀i ∈ 1, …, m.\,∃j ∈ 1, …, n.\,v_i ≃ v_j ∧ χ_i ≃ χ_j \\\\
           ∀j ∈ 1, …, n.\,∃i ∈ 1, …, m.\,v_i ≃ v_j ∧ χ_i ≃ χ_j}
          {\many{v_i ⇒ χ_i}{i < m} ≃ \many{v_j ⇒ χ_j}{j < n}} \\
        \inferrule[eq-fix-px]
          {∀i ∈ 1, …, m.\,(\mfix\;f\;(x{:}τ_1) : τ_2 = e)\;v_i ⟶^* v ∧ v ≃ χ_i}
          {\mfix\;f\;(x{:}τ_1) : τ_2 = e ≃ \many{v_i ⇒ χ_i}{i < m}} \\
        \inferrule[eq-ctor]
          {v_{11} ≃ v_{21} \;…\; v_{1k} ≃ v_{2k}}
          {C(v_{11}, …, v_{1k}) ≃ C(v_{21}, …, v_{2k})}
    \end{gather*}
  \end{center}
  \hrule
  \caption{\mlsyn{} evaluation and compatibility rules}
  \label{fig:mlsyn-eval}
\end{figure}
